dice: dpe: match syntax in derive_child. invoke actual engine code in DICEEngine.fst from dpe. current roadblock dynamically allocating global state and working with permissions on polymorphic record types

share/steel/examples/pulse/dice/engine/EngineCore.fst
@@ -11,6 +11,7 @@ module T = FStar.Tactics
 module US = FStar.SizeT
 module U8 = FStar.UInt8
 open Array
+open CommonTypes
 open EngineTypes
 open HACL
 
@@ -30,44 +31,44 @@ val uds_is_enabled : vprop
 assume
 val stack_is_erased : vprop
 
-let l0_is_authentic (vl0:l0_repr) 
+let l0_is_authentic (repr:engine_record_repr) 
   : prop
   = spec_ed25519_verify 
-      vl0.l0_image_auth_pubkey 
-      vl0.l0_image_header 
-      vl0.l0_image_header_sig /\
-    spec_hash dice_hash_alg vl0.l0_binary == vl0.l0_binary_hash
+      repr.l0_image_auth_pubkey 
+      repr.l0_image_header 
+      repr.l0_image_header_sig /\
+    spec_hash dice_hash_alg repr.l0_binary == repr.l0_binary_hash
 
-let cdi_functional_correctness (c0:Seq.seq U8.t) (vl0:l0_repr)
+let cdi_functional_correctness (c0:Seq.seq U8.t) (repr:engine_record_repr)
   : prop 
-  = c0 == spec_hmac dice_hash_alg (spec_hash dice_hash_alg uds_bytes) (spec_hash dice_hash_alg vl0.l0_binary)
+  = c0 == spec_hmac dice_hash_alg (spec_hash dice_hash_alg uds_bytes) (spec_hash dice_hash_alg repr.l0_binary)
 
 ```pulse
-fn authenticate_l0_image (l0:l0_image_t) (#vl0:Ghost.erased l0_repr)
-    requires l0_perm l0 vl0
+fn authenticate_l0_image (record:engine_record_t) (#repr:Ghost.erased engine_record_repr)
+    requires engine_record_perm record repr
     returns b:bool
     ensures (
-        l0_perm l0 vl0 **
-        pure (b ==> l0_is_authentic vl0)
+        engine_record_perm record repr **
+        pure (b ==> l0_is_authentic repr)
     )
 {
-  unfold l0_perm l0 vl0;
+  unfold engine_record_perm record repr;
 
   let valid_header_sig = ed25519_verify
-                          l0.l0_image_auth_pubkey
-                          l0.l0_image_header l0.l0_image_header_size
-                          l0.l0_image_header_sig;
+                          record.l0_image_auth_pubkey
+                          record.l0_image_header record.l0_image_header_size
+                          record.l0_image_header_sig;
   
   let mut b = false;
   if valid_header_sig {
     let hash_buf = new_array 0uy dice_digest_len;
-    hacl_hash dice_hash_alg l0.l0_binary l0.l0_binary_size hash_buf;
-    let res = compare dice_digest_len hash_buf l0.l0_binary_hash;
+    hacl_hash dice_hash_alg record.l0_binary record.l0_binary_size hash_buf;
+    let res = compare dice_digest_len hash_buf record.l0_binary_hash;
     free_array hash_buf;
-    fold l0_perm l0 vl0;
+    fold engine_record_perm record repr;
     res
   } else {
-    fold l0_perm l0 vl0;
+    fold engine_record_perm record repr;
     false
   };
 }
@@ -109,73 +110,109 @@ val read_uds (uds:A.larray U8.t (US.v uds_len))
       (fun _ -> A.pts_to uds full_perm uds_bytes `star` uds_is_enabled)
 
 ```pulse
-fn compute_cdi (c:cdi_t) (l0:l0_image_t) 
-               (#vl0:Ghost.erased l0_repr)
+fn compute_cdi (cdi:cdi_t) (uds:A.larray U8.t (US.v uds_len)) (record:engine_record_t) 
+               (#repr:Ghost.erased engine_record_repr)
                (#c0:Ghost.erased (Seq.seq U8.t))
   requires (
     uds_is_enabled **
-    A.pts_to c full_perm c0 **
-    l0_perm l0 vl0 (* should CDI only be computed on authentic l0 images? *)
+    A.pts_to uds full_perm uds_bytes **
+    A.pts_to cdi full_perm c0 **
+    engine_record_perm record repr (* should CDI only be computed on authentic l0 images? *)
   )
   ensures (
-    l0_perm l0 vl0 **
+    uds_is_enabled **
+    engine_record_perm record repr **
+    A.pts_to uds full_perm uds_bytes **
     exists (c1:Seq.seq U8.t). (
-      A.pts_to c full_perm c1 **
-      pure (cdi_functional_correctness c1 vl0))
+      A.pts_to cdi full_perm c1 **
+      pure (cdi_functional_correctness c1 repr))
   )
 {
-    let uds = new_array 0uy uds_len;
+    // let uds = new_array 0uy uds_len;
     let uds_digest = new_array 0uy dice_digest_len;
     let l0_digest = new_array 0uy dice_digest_len;
-    read_uds uds;
+    // read_uds uds;
     hacl_hash dice_hash_alg uds uds_len uds_digest;
 
-    unfold l0_perm l0 vl0;
-    hacl_hash dice_hash_alg l0.l0_binary l0.l0_binary_size l0_digest;
-    fold l0_perm l0 vl0;
+    unfold engine_record_perm record repr;
+    hacl_hash dice_hash_alg record.l0_binary record.l0_binary_size l0_digest;
+    fold engine_record_perm record repr;
 
     dice_digest_len_is_hashable;
 
-    hacl_hmac dice_hash_alg c 
+    hacl_hmac dice_hash_alg cdi 
       uds_digest dice_digest_len
       l0_digest dice_digest_len;
 
-    zeroize_uds uds uds_len;
-
     free_array l0_digest;
     free_array uds_digest;
-    free_array uds;
-    disable_uds();
+    // free_array uds;
     ()
 }
 ```
 
+#set-options "--print_implicits --print_universes"
+// ```pulse
+// fn engine_main (cdi:cdi_t) (ctxt:(t:context_t{Engine_context? t})) (record:engine_record_t)
+//                (#c0:Ghost.erased (Seq.seq U8.t))
+//                (#repr:Ghost.erased engine_record_repr)
+//   requires (
+//     uds_is_enabled **
+//     A.pts_to cdi full_perm c0 **
+//     engine_record_perm record repr
+//   )
+//   returns opt: option context_t
+//   ensures exists (c1:Seq.seq U8.t). (
+//       A.pts_to cdi full_perm c1 **
+//       engine_record_perm record repr **
+//       pure (Some? opt ==> l0_is_authentic repr /\ cdi_functional_correctness c1 repr)
+//   )
+// {
+//   let b = authenticate_l0_image record;
+//   if b 
+//   {
+//     compute_cdi cdi ctxt.uds record;
+//     Some (mk_l0_context cdi)
+//   }
+//   else
+//   {
+//     disable_uds ();
+//     None #context_t
+//   }
+// }
+// ```
 ```pulse
-fn dice_main (c:cdi_t) (l0:l0_image_t)
-             (#vl0:Ghost.erased l0_repr)
-             (#c0:Ghost.erased (Seq.seq U8.t))
+fn engine_main (cdi:cdi_t) (uds:A.larray U8.t (US.v uds_len)) (record:engine_record_t)
+               (#c0:Ghost.erased (Seq.seq U8.t))
+               (#repr:Ghost.erased engine_record_repr)
   requires (
     uds_is_enabled **
-    A.pts_to c full_perm c0 **
-    l0_perm l0 vl0
+    A.pts_to uds full_perm uds_bytes **
+    A.pts_to cdi full_perm c0 **
+    engine_record_perm record repr
   )
-  returns r: dice_return_code
-  ensures exists (c1:Seq.seq U8.t). (
-      A.pts_to c full_perm c1 **
-      l0_perm l0 vl0 **
-      pure (r == DICE_SUCCESS ==> l0_is_authentic vl0 /\ cdi_functional_correctness c1 vl0)
-  )
+  returns opt: option context_t
+  ensures (
+    engine_record_perm record repr **
+    A.pts_to uds full_perm (Seq.create (US.v uds_len) 0uy) **
+    exists (c1:Seq.seq U8.t). (
+      A.pts_to cdi full_perm c1 **
+      pure (Some? opt ==> l0_is_authentic repr /\ cdi_functional_correctness c1 repr)
+  ))
 {
-  let b = authenticate_l0_image l0;
+  let b = authenticate_l0_image record;
   if b 
   {
-    compute_cdi c l0;
-    DICE_SUCCESS
+    compute_cdi cdi uds record;
+    zeroize_uds uds uds_len;
+    disable_uds();
+    Some (mk_l0_context cdi)
   }
   else
   {
+    zeroize_uds uds uds_len;
     disable_uds ();
-    DICE_ERROR
+    None #context_t
   }
 }
 ```
