share/steel/examples/pulse/dice/engine/EngineTypes.fst
@@ -18,7 +18,7 @@ type dice_return_code = | DICE_SUCCESS | DICE_ERROR
 let cdi_t = A.larray U8.t (US.v (digest_len dice_hash_alg))
 
 noeq
-type l0_image_t = {
+type engine_record_t = {
   l0_image_header_size : signable_len;
   l0_image_header      : A.larray U8.t (US.v l0_image_header_size);
   l0_image_header_sig  : A.larray U8.t 64; (* secret bytes *)
@@ -27,9 +27,13 @@ type l0_image_t = {
   l0_binary_hash       : A.larray U8.t (US.v dice_digest_len); (*secret bytes *)
   l0_image_auth_pubkey : A.larray U8.t 32; (* secret bytes *)
 }
+let mk_engine_record  l0_image_header_size l0_image_header l0_image_header_sig
+                      l0_binary_size l0_binary l0_binary_hash l0_image_auth_pubkey
+  = {l0_image_header_size; l0_image_header; l0_image_header_sig;
+     l0_binary_size; l0_binary; l0_binary_hash; l0_image_auth_pubkey}
 
 //[@@erasable] Could we make l0_repr erasable from the get go?
-type l0_repr = {
+type engine_record_repr = {
     l0_image_header      : Seq.seq U8.t;
     l0_image_header_sig  : Seq.seq U8.t;
     l0_binary            : Seq.seq U8.t;
@@ -37,10 +41,10 @@ type l0_repr = {
     l0_image_auth_pubkey : Seq.seq U8.t;
 }
 
-let l0_perm (l0:l0_image_t) (vl0: l0_repr) 
+let engine_record_perm (record:engine_record_t) (repr:engine_record_repr) 
   : vprop = 
-  A.pts_to l0.l0_image_header full_perm vl0.l0_image_header `star`
-  A.pts_to l0.l0_image_header_sig full_perm vl0.l0_image_header_sig `star`
-  A.pts_to l0.l0_binary full_perm vl0.l0_binary `star`
-  A.pts_to l0.l0_binary_hash full_perm vl0.l0_binary_hash `star`
-  A.pts_to l0.l0_image_auth_pubkey full_perm vl0.l0_image_auth_pubkey
+  A.pts_to record.l0_image_header full_perm repr.l0_image_header `star`
+  A.pts_to record.l0_image_header_sig full_perm repr.l0_image_header_sig `star`
+  A.pts_to record.l0_binary full_perm repr.l0_binary `star`
+  A.pts_to record.l0_binary_hash full_perm repr.l0_binary_hash `star`
+  A.pts_to record.l0_image_auth_pubkey full_perm repr.l0_image_auth_pubkey
