share/steel/examples/pulse/dice/common/CommonTypes.fst
@@ -1,0 +1,73 @@
+module CommonTypes
+module A = Steel.ST.Array
+module US = FStar.SizeT
+module U8 = FStar.UInt8
+module U32 = FStar.UInt32
+open HACL
+open EngineTypes
+open L0Types
+
+(* ----------- CONTEXT ----------- *)
+noeq
+type engine_context = { uds: A.array U8.t; }
+
+noeq
+type l0_context = { _cdi: A.array U8.t; }
+
+noeq
+type l1_context = { aliasKey_priv: A.larray U8.t 32;
+                    cert_aliasKey: A.array U8.t;
+                    csr_deviceID: A.array U8.t; }
+
+// noeq
+// type context_t = 
+//   | Engine_context  : uds:A.array U8.t -> 
+//                       context_t
+//   | L0_context      : cdi:A.array U8.t -> 
+//                       context_t
+//   | L1_context      : aliasKey_priv:A.larray U8.t 32 ->
+//                       cert_aliasKey:A.array U8.t ->
+//                       csr_deviceID:A.array U8.t ->
+//                       context_t
+
+noeq
+type context_t = 
+  | Engine_context :engine_context -> context_t
+  | L0_context     : c:l0_context -> context_t
+  | L1_context     : c:l1_context -> context_t
+
+let mk_engine_context uds = Engine_context { uds }
+let mk_l0_context _cdi = L0_context { _cdi }
+let mk_l1_context aliasKey_priv cert_aliasKey csr_deviceID = L1_context { aliasKey_priv; cert_aliasKey; csr_deviceID }
+
+
+
+(* ----------- RECORD ----------- *)
+
+noeq
+type l0_record_t = {
+  cdi: A.larray U8.t 32;
+  fwid: A.larray U8.t 32;
+  deviceID_label_len: hkdf_lbl_len; (* should be U32 *)
+  deviceID_label: A.larray U8.t (US.v deviceID_label_len); (* public bytes *)
+  aliasKey_label_len: hkdf_lbl_len; (* should be U32 *)
+  aliasKey_label: A.larray U8.t (US.v aliasKey_label_len); (* public bytes *)
+  deviceIDCSR_ingredients: deviceIDCSR_ingredients_t;
+  aliasKeyCRT_ingredients: aliasKeyCRT_ingredients_t;
+}
+let mk_l0_record  cdi fwid deviceID_label_len deviceID_label 
+                  aliasKey_label_len aliasKey_label 
+                  deviceIDCSR_ingredients aliasKeyCRT_ingredients 
+  = {cdi; fwid; deviceID_label_len; deviceID_label; 
+     aliasKey_label_len; aliasKey_label; 
+     deviceIDCSR_ingredients; aliasKeyCRT_ingredients}
+     
+noeq
+type record_t =
+  | Engine_record : r:engine_record_t -> record_t
+  | L0_record     : r:l0_record_t -> record_t
+
+noeq
+type repr_t = 
+  | Engine_repr : r:engine_record_repr -> repr_t
+  // | L0_repr : r:l0_record_repr -> repr_t
